

Applied Time Series

Bérénice Maire
Édouard Blanc

December 2025

Theoretical Exercises

Exercise 1: Stationarity

Let $\{\varepsilon_t\}_{t \in \mathbb{Z}}$ be a weak white noise with variance σ^2 :

$$\forall t, \quad \mathbb{E}(\varepsilon_t) = 0, \quad \text{Var}(\varepsilon_t) = \mathbb{E}(\varepsilon_t^2) = \sigma^2 < \infty, \quad \text{Cov}(\varepsilon_t, \varepsilon_{t-h}) = \mathbb{E}(\varepsilon_t \varepsilon_{t-h}) = 0 \quad (h \neq 0).$$

A process $\{X_t\}$ is weakly stationary if:

$$\mathbb{E}(X_t) \text{ is constant,}$$

$$\text{Var}(X_t) \text{ is constant,}$$

$$\text{Cov}(X_t, X_{t-h}) \text{ depends only on } h \text{ (not on } t\text{)}.$$

$$1) \quad y_t = \varepsilon_t - \varepsilon_{t-1}$$

$$\mathbb{E}(y_t) = 0.$$

$$\begin{aligned} \text{Var}(y_t) &= \text{Var}(\varepsilon_t - \varepsilon_{t-1}) \\ &= \text{Var}(\varepsilon_t) + \text{Var}(\varepsilon_{t-1}) - 2 \text{Cov}(\varepsilon_t, \varepsilon_{t-1}) \\ &= \sigma^2 + \sigma^2 - 0 = 2\sigma^2. \end{aligned}$$

For the autocovariance function, for $h \in \mathbb{Z}$,

$$\gamma_y(h) := \text{Cov}(y_t, y_{t-h}) = \text{Cov}(\varepsilon_t - \varepsilon_{t-1}, \varepsilon_{t-h} - \varepsilon_{t-h-1}).$$

Using that ε_t is weak white noise (uncorrelated over time), we get

$$\gamma_y(0) = 2\sigma^2, \quad \gamma_y(1) = \text{Cov}(y_t, y_{t-1}) = -\sigma^2, \quad \gamma_y(h) = 0 \text{ for } |h| > 1.$$

Hence $\gamma_y(h)$ depends only on h and y_t is weakly stationary (it is an MA(1)).

$$2) \quad z_t = a\varepsilon_t + b\varepsilon_{t-1}$$

$$\mathbb{E}(z_t) = 0, \quad \text{Var}(z_t) = a^2\sigma^2 + b^2\sigma^2 = \sigma^2(a^2 + b^2).$$

Moreover, for $h \in \mathbb{Z}$,

$$\gamma_z(h) := \text{Cov}(z_t, z_{t-h}) = \text{Cov}(a\varepsilon_t + b\varepsilon_{t-1}, a\varepsilon_{t-h} + b\varepsilon_{t-h-1}).$$

Thus,

$$\gamma_z(0) = \sigma^2(a^2 + b^2), \quad \gamma_z(1) = ab\sigma^2, \quad \gamma_z(h) = 0 \text{ for } |h| > 1,$$

so $\gamma_z(h)$ depends only on h and z_t is weakly stationary (MA(1)).

$$3) \quad \text{Random walk: } w_0 = 0, \quad w_t = w_{t-1} + \varepsilon_t \text{ for } t > 0$$

$$w_t = \sum_{j=1}^t \varepsilon_j \quad \Rightarrow \quad \mathbb{E}(w_t) = 0, \quad \text{Var}(w_t) = \sum_{j=1}^t \text{Var}(\varepsilon_j) = t\sigma^2.$$

The variance depends on t , so w_t is not weakly stationary.

Exercise 2: Transformation of a stationary process

Let $U_t = \mu + \sum_{k=0}^{\infty} \theta_k \varepsilon_{t-k}$, with $\sum_{k=0}^{\infty} |\theta_k| < \infty$.

1) Mean

$$\begin{aligned}\mathbb{E}(U_t) &= \mathbb{E}\left(\mu + \sum_{k=0}^{\infty} \theta_k \varepsilon_{t-k}\right) \\ &= \mathbb{E}(\mu) + \mathbb{E}\left(\sum_{k=0}^{\infty} \theta_k \varepsilon_{t-k}\right) \\ &= \mu + \sum_{k=0}^{\infty} \theta_k \mathbb{E}(\varepsilon_{t-k}) \\ &= \mu + \sum_{k=0}^{\infty} \theta_k \cdot 0 \\ &= \mu.\end{aligned}$$

2) Variance

$$\text{Var}(U_t) = \text{Var}\left(\sum_{k=0}^{\infty} \theta_k \varepsilon_{t-k}\right) = \sum_{k=0}^{\infty} \theta_k^2 \text{Var}(\varepsilon_{t-k}) = \sigma^2 \sum_{k=0}^{\infty} \theta_k^2.$$

3) Autocovariance $\gamma_h = \text{Cov}(U_t, U_{t-h})$, $h > 0$

Write

$$U_t - \mu = \sum_{k=0}^{\infty} \theta_k \varepsilon_{t-k}, \quad U_{t-h} - \mu = \sum_{j=0}^{\infty} \theta_j \varepsilon_{t-h-j}.$$

Then

$$\begin{aligned}\gamma_h &= \text{Cov}(U_t, U_{t-h}) = \mathbb{E}\left[(U_t - \mu)(U_{t-h} - \mu)\right] \\ &= \sum_{k=0}^{\infty} \sum_{j=0}^{\infty} \theta_k \theta_j \mathbb{E}(\varepsilon_{t-k} \varepsilon_{t-h-j}).\end{aligned}$$

Since $\{\varepsilon_t\}$ is a weak white noise,

$$\mathbb{E}(\varepsilon_{t-k} \varepsilon_{t-h-j}) = \begin{cases} \sigma^2, & \text{if } t-k = t-h-j, \\ 0, & \text{otherwise,} \end{cases}$$

i.e. it is non-zero only when $t-k = t-h-j \iff j = k-h$. Because $j \geq 0$, this requires $k \geq h$. Therefore,

$$\gamma_h = \sigma^2 \sum_{k=h}^{\infty} \theta_k \theta_{k-h}.$$

Now perform the index shift $m = k-h$ (so $k = m+h$):

$$\gamma_h = \sigma^2 \sum_{m=0}^{\infty} \theta_{m+h} \theta_m.$$

Hence γ_h depends only on h .

Exercise 3: Forecast error

$$X_t = 0.5 + 0.8X_{t-1} + \varepsilon_t, \quad (\phi = 0.8 < 1, \ c = 0.5).$$

1) Best linear forecast

We consider the AR(1):

$$X_t = c + \phi X_{t-1} + \varepsilon_t, \quad |\phi| < 1, \quad \mathbb{E}(\varepsilon_t \mid \Omega_{t-1}) = 0.$$

Let $\mu = \mathbb{E}(X_t)$. Taking expectations:

$$\mathbb{E}(X_t) = c + \phi \mathbb{E}(X_{t-1}) + \mathbb{E}(\varepsilon_t).$$

Since $\mathbb{E}(X_t) = \mathbb{E}(X_{t-1}) = \mu$ and $\mathbb{E}(\varepsilon_t) = 0$,

$$\mu = c + \phi\mu \quad \Rightarrow \quad (1 - \phi)\mu = c \quad \Rightarrow \quad \mu = \frac{c}{1 - \phi}.$$

Here $c = 0.5$ and $\phi = 0.8$, hence $\mu = 2.5$.

h -step-ahead forecast

Rewrite the process in deviations from the mean:

$$X_t - \mu = c + \phi X_{t-1} + \varepsilon_t - \mu.$$

Using $c = (1 - \phi)\mu$,

$$X_t - \mu = \phi(X_{t-1} - \mu) + \varepsilon_t.$$

Let $Y_t := X_t - \mu$. Then $Y_t = \phi Y_{t-1} + \varepsilon_t$.

1-step-ahead forecast

Taking conditional expectation given Ω_t :

$$\begin{aligned} \mathbb{E}(Y_{t+1} \mid \Omega_t) &= \mathbb{E}(\phi Y_t + \varepsilon_{t+1} \mid \Omega_t) \\ &= \phi Y_t + \underbrace{\mathbb{E}(\varepsilon_{t+1} \mid \Omega_t)}_{=0} \\ &= \phi Y_t. \end{aligned}$$

Thus

$$\mathbb{E}(X_{t+1} \mid \Omega_t) - \mu = \phi(X_t - \mu) \quad \Rightarrow \quad \mathbb{E}(X_{t+1} \mid \Omega_t) = \mu + \phi(X_t - \mu).$$

h -step-ahead forecast (iteration)

By iteration,

$$\mathbb{E}(Y_{t+h} \mid \Omega_t) = \phi^h Y_t \quad \Rightarrow \quad X_t^*(h) := \mathbb{E}(X_{t+h} \mid \Omega_t) = \mu + \phi^h(X_t - \mu).$$

Here,

$$X_t^*(h) = 2.5 + 0.8^h(X_t - 2.5), \quad h \rightarrow \infty : X_t^*(h) \rightarrow 2.5.$$

2) Forecast error

By definition,

$$e_t(h) = X_{t+h} - X_t^*(h).$$

Iterating the deviation equation gives

$$Y_{t+h} = \phi^h Y_t + \sum_{j=0}^{h-1} \phi^j \varepsilon_{t+h-j}.$$

Therefore,

$$e_t(h) = X_{t+h} - X_t^*(h) = \sum_{j=0}^{h-1} \phi^j \varepsilon_{t+h-j}.$$

3) Variance of forecast error

$$\begin{aligned} \text{Var}(e_t(h)) &= \text{Var}\left(\sum_{j=0}^{h-1} \phi^j \varepsilon_{t+h-j}\right) = \sum_{j=0}^{h-1} \phi^{2j} \text{Var}(\varepsilon_{t+h-j}) \\ &= \sigma_\varepsilon^2 \sum_{j=0}^{h-1} \phi^{2j} = \sigma_\varepsilon^2 \frac{1 - \phi^{2h}}{1 - \phi^2}. \end{aligned}$$

With $\phi = 0.8$,

$$\text{Var}(e_t(h)) = \sigma_\varepsilon^2 \frac{1 - 0.8^{2h}}{0.36}, \quad h \rightarrow \infty : \text{Var}(e_t(h)) \rightarrow \frac{\sigma_\varepsilon^2}{0.36}.$$

4) Prediction interval

Under normality, $e_t(h) \sim \mathcal{N}(0, \sigma_h^2)$ with $\sigma_h^2 = \text{Var}(e_t(h))$. Thus a $(1 - \alpha)$ prediction interval centered at $X_t^*(h)$ is

$$\text{CI}_\alpha(X_t^*(h)) = X_t^*(h) \pm z_{\alpha/2} \sigma_h.$$

$$\text{Using } \sigma_h^2 = \sigma_\varepsilon^2 \frac{1 - \phi^{2h}}{1 - \phi^2},$$

$$\text{CI}_\alpha(X_t^*(h)) = X_t^*(h) \pm z_{\alpha/2} \sqrt{\sigma_\varepsilon^2 \frac{1 - \phi^{2h}}{1 - \phi^2}}.$$

As $h \rightarrow \infty$,

$$\text{CI}_\alpha(X_t^*(h)) \rightarrow \mu \pm z_{\alpha/2} \sqrt{\frac{\sigma_\varepsilon^2}{1 - \phi^2}}.$$

Exercise 4: The MA(1)-GARCH(1) model

$$y_t = \theta_0 + \varepsilon_t + \theta_1 \varepsilon_{t-1}, \quad h_t = \text{Var}_{t-1}(\varepsilon_t) = \alpha_0 + \alpha_1 \varepsilon_{t-1}^2 + \alpha_2 h_{t-1}.$$

Let \mathcal{F}_{t-1} be the information set at time $t - 1$ and assume $\mathbb{E}(\varepsilon_t | \mathcal{F}_{t-1}) = 0$.

1) Conditional and unconditional mean

$$\mathbb{E}(y_t | \mathcal{F}_{t-1}) = \mathbb{E}(\theta_0 + \varepsilon_t + \theta_1 \varepsilon_{t-1} | \mathcal{F}_{t-1}) = \theta_0 + \theta_1 \varepsilon_{t-1}, \quad \mathbb{E}(y_t) = \theta_0.$$

2) Conditional and unconditional variance

Since $\mathbb{E}(y_t \mid \mathcal{F}_{t-1}) = \theta_0 + \theta_1 \varepsilon_{t-1}$,

$$y_t - \mathbb{E}(y_t \mid \mathcal{F}_{t-1}) = \varepsilon_t \quad \Rightarrow \quad \text{Var}_{t-1}(y_t) = \text{Var}_{t-1}(\varepsilon_t) = h_t.$$

For the unconditional variance, use $y_t - \mathbb{E}(y_t) = \varepsilon_t + \theta_1 \varepsilon_{t-1}$, hence

$$\text{Var}(y_t) = \text{Var}(\varepsilon_t) + \theta_1^2 \text{Var}(\varepsilon_{t-1}) + 2\theta_1 \text{Cov}(\varepsilon_t, \varepsilon_{t-1}).$$

In a (zero-mean) GARCH model, the innovations ε_t are uncorrelated over time, so $\text{Cov}(\varepsilon_t, \varepsilon_{t-1}) = 0$, and therefore

$$\text{Var}(y_t) = (1 + \theta_1^2) v,$$

where $v = \text{Var}(\varepsilon_t) = \mathbb{E}(h_t)$. Taking expectation in the GARCH recursion:

$$v = \alpha_0 + \alpha_1 v + \alpha_2 v \quad \Rightarrow \quad v = \frac{\alpha_0}{1 - \alpha_1 - \alpha_2} \quad (\alpha_1 + \alpha_2 < 1).$$

Hence

$$\text{Var}(y_t) = (1 + \theta_1^2) \frac{\alpha_0}{1 - \alpha_1 - \alpha_2}.$$